theories/MetaTheory/SubjectReduction.v
@@ -7,11 +7,10 @@ From Metaprog Require Export MetaTheory.Typing.
 (** Beta reduction preserves typing. *)
 Lemma typing_beta {s} Σ Γ x ty body arg args (T : term s) :
   typing_evar_map Σ ->
-  typing_context Σ Γ ->
   Σ ;; Γ ⊢ TApp (TLam x ty body) (arg :: args) : T ->
   Σ ;; Γ ⊢ TApp (body[x := arg]) args : T.
 Proof.
-intros HΣ HΓ H. pose proof (HT := typing_validity _ _ _ _ HΣ HΓ H).
+intros HΣ H. pose proof (HT := typing_validity _ _ _ _ HΣ H).
 apply typing_app_inv in H. destruct H as (f_ty & T' & H1 & H2 & H3).
 apply typing_conv_type with T' ; [|assumption..]. clear T H3 HT.
 
@@ -23,8 +22,9 @@ assert (Hbody' : Σ ;; Γ ⊢ body[x := arg] : body_ty[x := arg]).
 {
   apply typing_substitute with (CCons Γ x ty) ; [assumption|].
   apply typing_scons.
+  - assumption.
   - simpl_subst. apply typing_conv_type with a ; auto.
-  - apply typing_sid.
+  - apply typing_sid. eapply typing_context_validity ; eauto.
 }
 
 assert (Hbody'' : Σ ;; Γ ⊢ body[x := arg] : b[x := arg]).
@@ -33,7 +33,10 @@ assert (Hbody'' : Σ ;; Γ ⊢ body[x := arg] : b[x := arg]).
   - now rewrite Hb.
   - change TType with (TType[x := arg]). eapply typing_substitute with (CCons Γ x a).
     + apply typing_prod_inv in H. apply H.
-    + apply typing_scons ; [|apply typing_sid]. simpl_subst. assumption.
+    + apply typing_scons.
+      * eapply typing_validity ; eassumption.
+      * simpl_subst. assumption.
+      * apply typing_sid. eapply typing_context_validity ; eauto.
 }
 eapply typing_app ; eauto.
 Qed.
@@ -41,18 +44,20 @@ Qed.
 (** Evar expansion preserves typing. *)
 Lemma typing_evar_expand {s} Σ Γ ev ty def (T : term s) :
   typing_evar_map Σ ->
-  typing_context Σ Γ ->
   Σ ;; Γ ⊢ TEvar ev : T ->
   Σ ev = Some (mk_evar_entry ty (Some def)) ->
   Σ ;; Γ ⊢ wk def : T.
 Proof.
-intros HΣ HΓ Hev Hentry. apply typing_conv_type with (wk ty).
-- unfold wk. apply typing_rename with CNil.
+intros HΣ Hev Hentry. apply typing_conv_type with (wk ty).
+- simpl_subst. apply typing_rename with CNil.
   + apply HΣ in Hentry. depelim Hentry. assumption.
-  + intros i. depelim i.
+  + split3.
+    * constructor.
+    * eapply typing_context_validity ; eassumption.
+    * intros i. depelim i.
 - apply typing_evar_inv in Hev. destruct Hev as (entry & H & HT).
   rewrite H in Hentry. depelim Hentry. cbn in HT. now symmetry.
-- eapply typing_validity ; eauto.
+- eapply typing_validity ; eassumption.
 Qed.
 
 Reserved Notation "Σ ⊢ Γ1 '~>ctx' Γ2"
@@ -72,57 +77,137 @@ where "Σ ⊢ Γ1 '~>ctx' Γ2" := (red1_context Σ Γ1 Γ2).
 
 Derive Signature for red1_context.
 
-(*Lemma typing_red1_var {s} Σ Γ (i : index s) :
+
+Definition sr_prop Σ {s} Γ (t T : term s) :=
   typing_evar_map Σ ->
-  typing_context Σ Γ ->
-  forall Γ',
-    Σ ⊢ Γ ~>ctx Γ' ->
-    Σ ;; Γ' ⊢ TVar i : lookup_context i Γ.
+    (forall t', Σ ⊢ t ~> t' -> Σ ;; Γ ⊢ t' : T) /\
+    (forall Γ', Σ ⊢ Γ ~>ctx Γ' -> Σ ;; Γ' ⊢ t : T).
+
+Lemma All_context_and (P Q : forall s, context ∅ s -> term s -> term s -> Prop) s (Γ : context ∅ s) :
+  All_context (fun s Γ t T => P s Γ t T /\ Q s Γ t T) Γ <->
+  (All_context P Γ /\ All_context Q Γ).
 Proof.
-intros HΣ HΓ. induction HΓ ; intros Γ' Hred.
-- depelim Hred.
-- depelim Hred ; depelim i ; simp lookup_context ; simpl_subst.
-  + cbn in H1. depelim H1.
-    assert (Γ0 = Γ) as -> by admit.
-    assert (ty0 = ty) as -> by admit.
-    clear H1 H3 H3'.*)
+induction Γ.
+- split ; constructor ; constructor.
+- split.
+  + intros H. depelim H. rewrite IHΓ in H. split ; now constructor.
+  + intros (H1 & H2). depelim H1. depelim H2. constructor.
+    * now rewrite IHΓ.
+    * now split.
+Qed.
+
+Lemma red1_context_conv_lookup {s} Σ (Γ Γ' : context ∅ s) i :
+  Σ ⊢ Γ ~>ctx Γ' ->
+  Σ ⊢ lookup_context i Γ ≡ lookup_context i Γ'.
+Proof.
+intros Hred. induction Hred ; depelim i ; simp lookup_context ; simpl_subst.
+- now rewrite H.
+- reflexivity.
+- reflexivity.
+- now rewrite IHHred.
+Qed.
+
+Lemma typing_context_red1 {s} Σ (Γ Γ' : context ∅ s) :
+  typing_evar_map Σ ->
+  All_context (@sr_prop Σ) Γ ->
+  Σ ⊢ Γ ~>ctx Γ' ->
+  typing_context Σ Γ ->
+  typing_context Σ Γ'.
+Proof.
+intros HΣ Hsr Hred HΓ. induction Hred.
+- constructor.
+  + now depelim HΓ.
+  + depelim HΓ. depelim Hsr. now apply H.
+- constructor.
+  + apply IHHred.
+    * now depelim Hsr.
+    * now depelim HΓ.
+  + depelim Hsr. apply H ; auto.
+Qed.
+
+Lemma typing_lookup_context_red1 {s} Σ (Γ Γ' : context ∅ s) i :
+  typing_evar_map Σ ->
+  All_context (@sr_prop Σ) Γ ->
+  typing_context Σ Γ ->
+  Σ ⊢ Γ ~>ctx Γ' ->
+  Σ ;; Γ' ⊢ lookup_context i Γ : TType.
+Proof.
+intros HΣ Hsr HΓ Hred. induction Hred.
+- depelim Hsr. depelim HΓ. depelim i ; simp lookup_context ; simpl_subst.
+  + change TType with (rename (@rshift s x) TType). apply typing_rename with Γ ; auto.
+    apply typing_rshift. constructor ; auto. now apply H.
+  + change TType with (rename (@rshift s x) TType). apply typing_rename with Γ.
+    * now apply typing_lookup_context.
+    * apply typing_rshift. constructor ; auto. now apply H.
+- depelim Hsr. depelim HΓ. depelim i ; simp lookup_context ; simpl_subst.
+  + change TType with (rename (@rshift s x) TType). apply typing_rename with Γ' ; auto.
+    * now apply H.
+    * apply typing_rshift. constructor ; auto.
+      --apply typing_context_red1 with Γ ; auto.
+      --now apply H.
+  + change TType with (rename (@rshift s x) TType). apply typing_rename with Γ' ; auto.
+    apply typing_rshift. constructor ; auto.
+    --apply typing_context_red1 with Γ ; auto.
+    --now apply H.
+Qed.
+
+(** In [All_spine Σ P f_ty args T] we can change the function type [f_ty]
+    to a convertible one, as long as we are willing to accept that the return
+    type [T] also changes to a convertible one. *)
+Lemma All_spine_conv_func_type {s} Σ P f_ty f_ty' args (T : term s) :
+  All_spine Σ P f_ty args T ->
+  Σ ⊢ f_ty ≡ f_ty' ->
+  exists T',
+    All_spine Σ P f_ty' args T' /\
+    Σ ⊢ T ≡ T'.
+Proof.
+intros Hspine Hconv. induction Hspine in f_ty', Hconv |- *.
+- exists f_ty'. split ; [constructor | assumption].
+- specialize (IHHspine (b[x := arg])). forward IHHspine by reflexivity.
+  destruct IHHspine as (T' & Hspine' & HconvT).
+  exists T'. split ; auto. econstructor ; eauto. now rewrite <-Hconv.
+Qed.
+
+Lemma typing_spine_red1 {s} Σ (Γ : context ∅ s) f_ty args args' T :
+  typing_evar_map Σ ->
+  All_spine Σ (fun t T => Σ ;; Γ ⊢ t : T /\ sr_prop Σ Γ t T) f_ty args T ->
+  All2 (fun a a' => Σ ⊢ a ~> a' \/ a = a') args args' ->
+  exists T',
+    All_spine Σ (typing Σ Γ) f_ty args' T' /\
+    Σ ⊢ T ≡ T'.
+Proof.
+intros HΣ Hspine Hred. revert f_ty T Hspine. induction Hred ; intros f_ty T Hspine.
+- depelim Hspine. exists f_ty. split ; [constructor | reflexivity].
+- depelim Hspine. destruct H0 as (H0 & H0'). destruct H as [H | ->].
+  + destruct (IHHred _ _ Hspine) as (T' & HT' & Hconv).
+    apply All_spine_conv_func_type with (f_ty' := b[x0 := y]) in HT'.
+    * destruct HT' as (T'' & HT' & HT''). exists T''. split.
+      --econstructor ; eauto. now apply H2.
+      --now rewrite Hconv.
+    * admit.
+  + destruct (IHHred _ _ Hspine) as (T' & HT' & Hconv).
+    apply All_spine_conv_func_type with (f_ty' := b[x0 := y]) in HT'.
+    * destruct HT' as (T'' & HT' & HT''). exists T''. split.
+      --econstructor ; eauto. now destruct H2.
+      --now rewrite Hconv.
+    * reflexivity.
+Admitted.
 
 (** One-step reduction preserves typing. *)
-Lemma typing_red1_aux {s} Σ Γ (t T : term s) :
-  typing_evar_map Σ ->
-  typing_context Σ Γ ->
+Lemma typing_red1 {s} Σ Γ (t T : term s) :
   Σ ;; Γ ⊢ t : T ->
-  (forall t', Σ ⊢ t ~> t' -> Σ ;; Γ ⊢ t' : T) /\
-  (forall Γ', Σ ⊢ Γ ~>ctx Γ' -> Σ ;; Γ' ⊢ t : T).
+  sr_prop Σ Γ t T.
 Proof.
-intros HΣ HΓ Ht. induction Ht ; (split ; [intros t' Hred | intros Γ' Hred]).
+intros Ht. induction Ht ; (split ; [intros t' Hred | intros Γ' Hred]).
 - depelim Hred.
-- constructor.
+- constructor. rewrite All_context_and in H. now apply typing_context_red1 with Γ.
 - depelim Hred.
-- subst. apply typing_conv_type with (lookup_context i Γ').
-  + now constructor.
-  + admit.
-  +
-admit.
-  (*
-  H1 : Σ ;; Γ ⊢ ty : TType
-  H2 : Σ ;; CCons Γ x ty ⊢ TVar I0 : wk ty
-  Hred : CCons Γ x ty ~> Γ'
-  IH: forall ty', Σ ⊢ ty ~> ty' -> Σ ;; Γ ⊢ ty' : TType
-
-  Case 1:
-    CCons Γ x ty ~> CCons Γ x ty' because Σ ⊢ ty ~> ty'
-    We need to show:
-      Σ ;; CCons Γ x ty' ⊢ TVar I0 : wk ty
-
-
-
-
-  *)
-
-- constructor.
-  + now apply IHHt1.
-  + apply IHHt2 ; auto ; now constructor.
+- subst. rewrite All_context_and in H. apply typing_conv_type with (lookup_context i Γ').
+  + constructor.
+    * now apply typing_context_red1 with Γ.
+    * reflexivity.
+  + symmetry. now apply red1_context_conv_lookup.
+  + now apply typing_lookup_context_red1.
 - depelim Hred.
   + apply typing_conv_type with (TProd x ty' body_ty).
     * constructor.
@@ -130,8 +215,7 @@ admit.
       --apply IHHt2 ; auto ; now constructor.
     * now rewrite Hred.
     * constructor ; auto. eapply typing_validity ; eauto.
-      constructor ; auto.
-  + constructor ; auto. apply IHHt2 ; auto. now constructor.
+  + constructor ; auto. apply IHHt2 ; auto.
 - constructor.
   + now apply IHHt1.
   + apply IHHt2 ; auto ; now constructor.
@@ -139,33 +223,39 @@ admit.
   + constructor.
     * apply IHHt1 ; auto.
     * apply IHHt2 ; auto ; now constructor.
-  + constructor ; auto. apply IHHt2 ; auto. now constructor.
-- apply typing_app with f_ty ; [now apply IHHt |].
-  clear f Ht IHHt. induction H ; econstructor ; try eassumption.
-  + apply H ; auto.
-  + apply H1 ; auto.
+  + constructor ; auto. apply IHHt2 ; auto.
+- constructor.
+  + now apply IHHt1.
+  + apply IHHt2 ; auto ; now constructor.
 - depelim Hred.
   + eapply typing_beta ; eauto. apply typing_app with f_ty ; eauto.
     revert H. apply All_spine_consequence. firstorder.
   + apply typing_app with f_ty ; [now apply IHHt |].
     revert H. apply All_spine_consequence. firstorder.
   + apply typing_app with f_ty ; [assumption |].
-    clear f IHHt Ht. revert f_ty T H. induction H0.
-    * intros f_ty T H1. depelim H1. eapply All_spine_cons ; eauto.
-      --now destruct H0.
+    clear f IHHt Ht. revert args' H1. induction H ; intros args' Hone. ; depelim Hone.
+    * econstructor ; eauto.
+      --now destruct H.
       --apply H2 ; auto.
-      --
-    * intros f_ty T H. depelim H. econstructor ; eauto.
+      --admit.
+    * econstructor ; eauto.
       --now destruct H.
       --now destruct H2.
-- now constructor.
-- depelim Hred. rewrite H in H0. depelim H0. cbn. unfold wk. eapply typing_rename.
-  + apply HΣ in H. depelim H. eassumption.
-  + intros i. depelim i.
+- apply typing_app with f_ty ; [now apply IHHt |].
+  clear f Ht IHHt. induction H ; econstructor ; try eassumption.
+  + apply H ; auto.
+  + apply H2 ; auto.
+- depelim Hred. rewrite H0 in H2. depelim H2. cbn. simpl_subst. eapply typing_rename.
+  + apply H1 in H0. depelim H0. eassumption.
+  + split3.
+    * constructor.
+    * revert H. apply All_context_consequence. firstorder.
+    * intros i. depelim i.
+- constructor ; auto. rewrite All_context_and in H. now apply typing_context_red1 with Γ.
+- apply typing_conv_type with A ; auto. now apply IHHt1.
 - apply typing_conv_type with A ; auto.
   + now apply IHHt1.
   + now apply IHHt2.
-- apply typing_conv_type with A ; auto. now apply IHHt1.
 Admitted.
 
 
